examples/ghc/theories/JoinPointInvariantsInductive.v
@@ -1,0 +1,364 @@
+Require Import CoreSyn.
+Require Import Id.
+Require Import IdInfo.
+Require Import VarSet.
+Require Import BasicTypes.
+
+Require Import Coq.Lists.List.
+Require Import Coq.Bool.Bool.
+Require Import Coq.ZArith.BinInt.
+Require Import Psatz.
+
+Import ListNotations.
+
+Set Bullet Behavior "Strict Subproofs".
+
+Open Scope Z_scope.
+
+Require Import JoinPointInvariants.
+
+(* This lemma exists, but is Opaque. No good for us. *)
+Lemma  forallb_forall
+     : forall (A : Type) (f : A -> bool) (l : list A),
+       forallb f l = true <-> (forall x : A, In x l -> f x = true).
+Proof.
+  intros.
+  induction l.
+  * split; intro.
+    - intros. inversion H0.
+    - reflexivity.
+  * split; intro.
+    - simpl in H. rewrite andb_true_iff in H. destruct H.
+      rewrite IHl in H0.
+      intros. destruct H1.
+      + subst. assumption.
+      + intuition.
+    - simpl. rewrite andb_true_iff. split.
+      + apply H. left. reflexivity.
+      + intuition.
+Defined.
+
+
+(* Attempt one: An inductive predicate *)
+Inductive JoinPointsValid : CoreExpr -> Z -> VarSet -> Prop :=
+  | JPV_Var     : forall v n jps,
+    isJoinId v = false ->
+    JoinPointsValid (Var v) n jps
+  | JPV_JoinVar : forall v a n jps,
+    isJoinId_maybe v = Some a ->
+    a <= n ->
+    elemVarSet v jps = true ->
+    JoinPointsValid (Var v) n jps
+  | JPV_List    : forall l n jps, JoinPointsValid (Lit l) n jps
+  | JPV_App     : forall e1 e2 n jps,
+    JoinPointsValid e1 (n+1) jps ->     (* Tail-call-position *)
+    JoinPointsValid e2 0 emptyVarSet -> (* Non-tail-call position *)
+    JoinPointsValid (App e1 e2) n jps
+  | JPV_Lam     : forall v e n jps,
+    JoinPointsValid e 0 emptyVarSet -> (* Non-tail-call position *)
+    JoinPointsValid (Lam v e) n jps
+  | JPV_LetNonRec  : forall v rhs body n jps, 
+    isJoinId v = false ->
+    JoinPointsValid rhs 0 emptyVarSet ->            (* Non-tail-call position *)
+    JoinPointsValid body 0 (delVarSet jps v) ->     (* Tail-call-position *)
+    JoinPointsValid (Let (NonRec v rhs) body) n jps
+  | JPV_LetNonRecJP  : forall v a rhs body n jps, (* Shadowing *)
+    isJoinId_maybe v = Some a ->
+    GoodJoinRHS a rhs jps ->
+    JoinPointsValid body 0 (extendVarSet jps v) ->     (* Tail-call-position *)
+    JoinPointsValid (Let (NonRec v rhs) body) n jps
+  | JPV_LetRec  : forall pairs body n jps,
+    List.null pairs = false -> (* Not join-point-specific, could be its own invariant *)
+    (forall v rhs, In (v,rhs) pairs -> isJoinId v = false) ->
+    (forall v rhs, In (v,rhs) pairs -> JoinPointsValid rhs 0 emptyVarSet)  -> (* Non-tail-call position *)
+    let jps' := delVarSetList jps (map fst pairs) in
+    JoinPointsValid body 0 jps' ->     (* Tail-call-position *)
+    JoinPointsValid (Let (Rec pairs) body) n jps
+  | JPV_LetRecJP  : forall pairs body n jps, 
+    List.null pairs = false -> (* Not join-point-specific, could be its own invariant *)
+    (forall v rhs, In (v,rhs) pairs -> isJoinId v = true) ->
+    let jps' := extendVarSetList jps (map fst pairs) in
+    (forall v rhs a, In (v,rhs) pairs ->
+                     isJoinId_maybe v = Some a ->
+                     GoodJoinRHS a rhs jps')  -> (* Non-tail-call position *)
+    JoinPointsValid body 0 jps' ->     (* Tail-call-position *)
+    JoinPointsValid (Let (Rec pairs) body) n jps
+  | JPV_Case  : forall scrut bndr ty alts n jps, 
+    JoinPointsValid scrut 0 emptyVarSet -> (* Non-tail-call position *)
+    let jps' := delVarSet jps bndr in
+    (forall dc pats rhs, In (dc,pats,rhs) alts ->
+                         let jps' := delVarSetList jps pats in
+                         JoinPointsValid rhs 0 jps')  -> (* Tail-call position *)
+    JoinPointsValid (Case scrut bndr ty alts) n jps
+  | JPV_Cast  : forall e co n jps, 
+    JoinPointsValid e 0 jps ->
+    JoinPointsValid (Cast e co) n jps
+  | JPV_Tick  : forall tickish e n jps, 
+    JoinPointsValid e 0 jps ->
+    JoinPointsValid (Tick tickish e) n jps
+  | JPV_Type  : forall ty n jps, 
+    JoinPointsValid (Type_ ty) n jps
+  | JPV_Coercion  : forall co n jps, 
+    JoinPointsValid (Coercion co) n jps
+ with
+  GoodJoinRHS : Z -> CoreExpr -> VarSet -> Prop :=
+  | GJR_Lam : forall a v e jps,
+    0 < a ->
+    GoodJoinRHS (a - 1) e (delVarSet jps v) ->
+    GoodJoinRHS a (Lam v e) jps
+  | GJR_RHS: forall a e jps,
+    a = 0 ->
+    JoinPointsValid e 0 jps->     (* Tail-call-position *)
+    GoodJoinRHS a e jps
+  .
+
+(* Attempt two: An executable checker *)
+
+
+(* Relating the two definitions (may not be needed or useful) *)
+
+Scheme JPV_mut := Induction for JoinPointsValid Sort Prop
+with GJR_mut := Induction for GoodJoinRHS Sort Prop.
+
+Axiom isJoinId_eq : forall v,
+  isJoinId v = match isJoinId_maybe v with | None => false |Some _ => true end.
+
+Axiom delVarList_singleton: forall jps v,
+  delVarSetList jps (v :: nil) = delVarSet jps v.
+
+Axiom extendVarList_singleton: forall jps v,
+  extendVarSetList jps (v :: nil) = extendVarSet jps v.
+
+Lemma bindersOf_cleanup:
+  forall {a b} (pairs : list (a * b)),
+  flat_map (fun '(binder, _) => binder :: nil) pairs = map fst pairs.
+Proof. intros.  induction pairs. reflexivity. destruct a0. simpl. rewrite IHpairs. reflexivity. Qed.
+
+Lemma JoinPointsValid_isJoinPointsValid:
+  forall e n jps,
+  JoinPointsValid e n jps -> isJoinPointsValid e n jps = true.
+Proof.
+  eapply JPV_mut with
+    (P0 := fun a rhs jps _ => 
+      (if a =? 0
+        then isJoinPointsValid rhs 0 jps 
+        else isJoinRHS a rhs jps) = true);
+  intros; simpl;
+  rewrite ?isJoinId_eq in *;
+  rewrite ?orb_true_iff, ?andb_true_iff in *;
+  rewrite ?bindersOf_cleanup.
+  * destruct (isJoinId_maybe v); congruence.
+  * rewrite e, andb_true_iff, Z.leb_le. split; assumption.
+  * reflexivity.
+  * split; assumption.
+  * assumption.
+  * destruct (isJoinId_maybe v); inversion_clear e.
+    split; assumption.
+  * rewrite e in *; clear e.
+    split; assumption.
+  * split; split.
+    - rewrite negb_true_iff.
+      assumption.
+    - rewrite orb_true_iff. left.
+      rewrite forallb_forall.
+      intros [v rhs] HIn.
+      erewrite e0 by eassumption.
+      reflexivity.
+    - rewrite forallb_forall.
+      intros [v rhs] HIn.
+      specialize (e0 _ _ HIn).
+      rewrite isJoinId_eq in e0.
+      destruct (isJoinId_maybe v); inversion_clear e0.
+      specialize (H _ _ HIn).
+      assumption.
+    - enough (Htmp : (forallb (fun p : Var.Var * Expr CoreBndr => isJoinId (fst p)) pairs) = false)
+         by (rewrite Htmp; assumption).
+      apply not_true_is_false. intro Hforallb.
+      rewrite forallb_forall in Hforallb.
+      destruct pairs; only 1: inversion e.
+      destruct p as [v rhs].
+      specialize (e0 v rhs (or_introl eq_refl)).
+      specialize (Hforallb (v, rhs) (or_introl eq_refl)).
+      simpl in Hforallb.
+      congruence.
+  * assert (Hforallb: forallb (fun p : Var.Var * Expr CoreBndr => isJoinId (fst p)) pairs = true).
+    { rewrite forallb_forall.
+      intros [v rhs] HIn.
+      erewrite e0 by eassumption.
+      reflexivity. }
+    rewrite Hforallb. clear Hforallb.
+    split; split.
+    - rewrite negb_true_iff.
+      assumption.
+    - rewrite orb_true_iff. right.
+      reflexivity.
+    - rewrite forallb_forall.
+      intros [v rhs] HIn.
+      specialize (e0 _ _ HIn).
+      rewrite isJoinId_eq in e0.
+      destruct (isJoinId_maybe v) eqn:HiJI; inversion_clear e0.
+      specialize (H _ _ _ HIn HiJI).
+      assumption.
+    - rewrite ?orb_true_iff, ?andb_true_iff in *.
+      assumption.
+  * split.
+    - assumption.
+    - rewrite forallb_forall.
+      intros [[dc pats] rhs] HIn.
+      eapply H0; eassumption.
+  * assumption.
+  * assumption.
+  * reflexivity.
+  * reflexivity.
+  * destruct (Z.eqb_spec a 0); try lia.
+    destruct (Z.ltb_spec a 1); try lia. 
+    destruct (Z.eqb_spec a 1).
+    - destruct (Z.eqb_spec (a-1) 0); try lia.
+      assumption.
+    - destruct (Z.eqb_spec (a-1) 0); try lia.
+      assumption.
+  * destruct (Z.eqb_spec a 0); try lia.
+    assumption.
+Qed.
+
+Lemma isJoinRHS_a_nonneg:
+  forall a rhs jps, isJoinRHS a rhs jps = true -> 0 <= a.
+Proof.
+  intros.
+  induction rhs; simpl in H; destruct (Z.ltb_spec a 1); try congruence.
+  lia.
+Qed.
+
+Lemma isJoinPointsValid_JoinPointsValid:
+  forall e n jps,
+  isJoinPointsValid e n jps = true -> JoinPointsValid e n jps.
+Proof.
+  refine (fix IH e n jps (H : isJoinPointsValid e n jps = true)  {struct e} : JoinPointsValid e n jps := _
+           with IHrhs a rhs jps (Hnn : a <> 0) (H : isJoinRHS a rhs jps = true) {struct rhs} : GoodJoinRHS a rhs jps := _
+           for IH).
+  * intros. destruct e; simpl in H; rewrite ?andb_true_iff in *.
+    - destruct (isJoinId_maybe i) eqn:?.
+      + rewrite ?andb_true_iff in *. destruct H.
+        rewrite Z.leb_le in *.
+        eapply JPV_JoinVar; try eassumption.
+      + assert (isJoinId i = false) by (rewrite isJoinId_eq; rewrite Heqo; reflexivity).
+        eapply JPV_Var; try eassumption.
+   - constructor.
+   - constructor; intuition.
+   - constructor; intuition.
+   - destruct b as [v rhs | pairs].
+     + rewrite isJoinId_eq in H.
+       destruct (isJoinId_maybe v) eqn:HJI; rewrite ?andb_true_iff in *.
+       ** eapply JPV_LetNonRecJP.
+          -- eassumption.
+          -- destruct (Z.eqb_spec j 0).
+             ++ eapply GJR_RHS; intuition.
+             ++ apply IHrhs; intuition.
+          -- apply IH; intuition.
+       ** eapply JPV_LetNonRec.
+          -- rewrite isJoinId_eq. rewrite HJI. reflexivity.
+          -- intuition.
+          -- intuition.
+     + (* We must be careful to call IH and IHrhs only on arguments that
+          are obviously elements of [pair], otherwise Coq will not accept
+          this proof as structurally termination. *)
+       assert (IH': forall v e n jps, In (v,e) pairs -> isJoinPointsValid e n jps = true -> JoinPointsValid e n jps).
+       { clear -IH.
+         intros. induction pairs; destruct H.
+         - destruct a. specialize (IH e0 n jps). inversion H. subst; intuition.
+         - intuition.
+       }
+       assert (IHrhs': forall v a rhs jps, In (v,rhs) pairs -> a <> 0 -> isJoinRHS a rhs jps = true -> GoodJoinRHS a rhs jps).
+       { clear -IHrhs.
+         intros. induction pairs; destruct H.
+         - destruct a0. specialize (IHrhs a e jps). inversion H. subst; intuition.
+         - intuition.
+       }
+
+      rewrite ?andb_true_iff in *.
+       destruct H as [[??][??]].
+       rewrite ?orb_true_iff in H0. destruct H0.
+       ** rewrite negb_true_iff in H.
+          rewrite forallb_forall in H0.
+          rewrite forallb_forall in H1.
+
+          assert (Hforallb : forallb (fun p : Var.Var * Expr CoreBndr => isJoinId (fst p)) pairs = false).
+          {
+             apply not_true_is_false. intro Hforallb.
+             rewrite forallb_forall in Hforallb.
+             destruct pairs; only 1: inversion H.
+             destruct p as [v rhs].
+             specialize (H0 (v, rhs) (or_introl eq_refl)).
+             specialize (Hforallb (v, rhs) (or_introl eq_refl)).
+             simpl in H0, Hforallb.
+             rewrite negb_true_iff in H0.
+             congruence.
+          }
+
+          eapply JPV_LetRec.
+          -- assumption.
+          -- intros v rhs HIn.
+             specialize (H0 (v,rhs) HIn).
+             rewrite negb_true_iff in H0.
+             apply H0.
+          -- intros v rhs HIn.
+             specialize (H0 (v,rhs) HIn).
+             rewrite negb_true_iff in H0. simpl in H0.
+             rewrite isJoinId_eq in H0.
+             specialize (H1 (v,rhs) HIn). simpl in H1.
+             destruct (isJoinId_maybe v) eqn:HJI; inversion_clear H0.
+             eapply IH'; eassumption.
+          -- rewrite Hforallb in H2.
+             eapply IH; eassumption.
+       ** rewrite negb_true_iff in H.
+          pose proof H0 as Hforallb. (* need this later *)
+          rewrite forallb_forall in H0.
+          rewrite forallb_forall in H1.
+
+          eapply JPV_LetRecJP.
+          -- assumption.
+          -- intros v rhs HIn.
+             specialize (H0 (v,rhs) HIn).
+             apply H0.
+          -- intros v rhs a HIn HJI.
+             specialize (H0 (v,rhs) HIn).
+             simpl in H0.
+             rewrite isJoinId_eq in H0.
+             specialize (H1 (v,rhs) HIn). simpl in H1.
+             rewrite HJI in *.
+             rewrite Hforallb in *.
+             destruct (Z.eqb_spec a 0).
+             ++ eapply GJR_RHS; try assumption.
+                eapply IH'; eassumption.
+             ++ eapply IHrhs'; eassumption.
+          -- rewrite Hforallb in *.
+             apply IH; assumption.
+   - destruct H.
+   
+     (* We must be careful to call IH and IHrhs only on arguments that
+        are obviously elements of [pair], otherwise Coq will not accept
+        this proof as structurally termination. *)
+     assert (IH': forall dc pats e n jps, In (dc,pats,e) l -> isJoinPointsValid e n jps = true -> JoinPointsValid e n jps).
+     { clear -IH.
+       intros. induction l; destruct H.
+       - destruct a as [[dc' pats'] e']. specialize (IH e' n jps). inversion H. subst; intuition.
+       - intuition.
+     }   
+   
+     constructor.
+     + apply IH; assumption.
+     + intros dc pats rhs Hin.
+       rewrite forallb_forall in H0.
+       specialize (H0 (dc, pats, rhs) Hin). simpl in H0.
+                Guarded.
+       eapply IH'; eassumption.
+   - constructor; intuition.
+   - constructor; intuition.
+   - constructor; intuition.
+   - constructor; intuition.
+ * destruct rhs; simpl in H; destruct (Z.ltb_spec a 1); try congruence.
+   eapply GJR_Lam. lia.
+   destruct (Z.eqb_spec a 1).
+   + apply GJR_RHS. lia. apply IH. assumption.
+   + apply IHrhs. lia. assumption. 
+Qed.
